ADTRefinement/Pick.v
@@ -7,26 +7,18 @@ Set Implicit Arguments.
 (** Every spec is trivially implementable using [Pick]. *)
 Section pick.
   Variable rep : Type.
-  Variable mutatorMethodContext : Context.
-  Variable observerMethodContext : Context.
-  Variable mutatorMethodSpecs : forall name, @mutatorMethodSpec rep mutatorMethodContext observerMethodContext name.
-  Variable observerMethodSpecs : forall name, @observerMethodSpec rep mutatorMethodContext observerMethodContext name.
+  Variable methodNames : Context.
+  Variable methodSpecs : forall name, @methodSpec rep methodNames name.
 
   Local Obligation Tactic := econstructor; eauto.
 
   Program Definition pickImpl : ADT :=
     {|
       Rep := rep;
-      MutatorContext := mutatorMethodContext;
-      ObserverContext := observerMethodContext;
-      UnbundledMutatorMethods idx :=
+      MethodNames := methodNames;
+      UnbundledMethods idx :=
         fun r x =>
           { r' : rep * cod _
-          | mutatorMethodSpecs idx r x (fst r') (snd r')}%comp;
-      UnbundledObserverMethods idx :=
-        fun r n =>
-          { n' : cod _
-          | observerMethodSpecs idx r n n'}%comp
+          | methodSpecs idx r x (fst r') (snd r')}%comp
     |}.
-
 End pick.
