ADTRefinement/Specs.v
@@ -2,21 +2,12 @@ Require Import Computation.
 
 Set Implicit Arguments.
 
-(* Specification of mutator method. *)
-Definition mutatorMethodSpec (Ty : Type)
-           (mutCtx obsCtx : Context)
-           (idx : @names mutCtx)
+(* Specification of method. *)
+Definition methodSpec (Ty : Type)
+           (indices : Context)
+           (idx : names)
   := Ty    (* Initial model *)
      -> dom idx (* Actual argument*)
      -> Ty (* Final Model *)
-     -> cod idx (* Return value *)
-     -> Prop.
-
-(* Specification of an observer method *)
-Definition observerMethodSpec (Ty : Type)
-           (mutCtx obsCtx : Context)
-           (idx : @names obsCtx)
-  := Ty    (* Initial model *)
-     -> dom idx (* Actual argument*)
      -> cod idx (* Return value *)
      -> Prop.
